Total/Stlc/Lang/Annotated/Semantics.lean
@@ -8,24 +8,30 @@ set_option autoImplicit false
 
 namespace Total.Stlc.Lang.Annotated
   namespace PrimOp
-    inductive Eval₁: (α: Nat) → (π: Domain Ty α) → (τ: Ty) → PrimOp α π τ → Term τ → Prop where
+    inductive Eval₁: {α: Nat} → {δ: Domain α} → {τ: Ty} → PrimOp δ τ → Args δ → Term τ → Prop where
   end PrimOp
 
   namespace Term
-    inductive IsValue: (τ: Ty) → Term τ → Prop where
-      | bool (b: Bool): IsValue .bool (.bool b)
-      | nat  (n: Nat):  IsValue .nat (.nat n)
-      -- | var (id: Ident): IsValue τ (.var id)
-      -- | abs {α: Nat} {π: Params Ty α} {τ: Ty} (formals: Params Ident Ty α π) (body: Term τ): IsValue (.fn π τ) (.abs formals body)
+    inductive IsValue: {τ: Ty} → Term τ → Prop where
+      | bool (b: Bool): IsValue (.bool b)
+      | nat  (n: Nat):  IsValue (.nat n)
 
-    inductive Eval₁ (τ: Ty): Term τ → Term τ → Prop where
+    abbrev Values {α: Nat} (δ: Domain α) := _root_.Values Term IsValue δ
 
-    def Eval (τ: Ty) := RTC (Eval₁ τ)
+    inductive Eval₁: {τ: Ty} → Term τ → Term τ → Prop where
+
+    abbrev Eval {τ: Ty}: Term τ → Term τ → Prop := RTC Eval₁
+
+    #check (.nil (.bool true) : Args (.nil .bool))
+    #check (.cons (.nat 2) (.cons (.nat 2) (.nil (.bool true))) : Args (.cons .nat (.cons .nat (.nil .bool))))
+
+    #check (.nil (.bool true): Values (.nil .bool))
+    #check (.cons (.nat 2) /- (.cons (.nat 2) (.nil (.bool true))) -/ : Values (.cons .nat (.cons .nat (.nil .bool))))
   end Term
 
   namespace Top
-    inductive IsValue (τ: Ty): Top τ → Prop where
-    inductive Eval₁ (τ: Ty): Top τ → Top τ → Prop where
-    def Eval (τ: Ty) := RTC (Eval₁ τ)
+    inductive IsValue: {τ: Ty} → Top τ → Prop where
+    inductive Eval₁: {τ: Ty} → Top τ → Top τ → Prop where
+    abbrev Eval {τ: Ty}: Top τ → Top τ → Prop := RTC Eval₁
   end Top
 end Total.Stlc.Lang.Annotated
