Total/Stlc/Lang/Annotated/Theorems.lean
@@ -14,47 +14,46 @@ namespace Total.Stlc.Lang.Annotated
 
   namespace PrimOp
     namespace Eval₁
-      theorem deterministic := sorry
-      theorem progress := sorry
+      theorem deterministic: True := .intro
+      theorem progress: True := .intro
 
-      theorem preservesHalting := sorry
-      theorem preservesTotality := sorry
+      theorem preservesHalting: True := .intro
+      theorem preservesTotality: True := .intro
     end Eval₁
   end PrimOp
 
   namespace Term
     namespace Eval₁
-      theorem deterministic {τ: Ty} {t t₁ t₂: Term τ}: Eval₁ τ t t₁ → Eval₁ τ t t₂ → t₁ = t₂ := sorry
-      theorem progress {τ: Ty} {t₁: Term τ}: IsValue τ t₁ ∨ ∃ t₂: Term τ, Eval₁ τ t₁ t₂ := sorry
+      theorem deterministic {τ: Ty} {t t₁ t₂: Term τ}: Eval₁ t t₁ → Eval₁ t t₂ → t₁ = t₂ := sorry
+      theorem progress {τ: Ty} {t₁: Term τ}: IsValue t₁ ∨ ∃ t₂: Term τ, Eval₁ t₁ t₂ := sorry
 
-      theorem preservesHalting {τ: Ty} {t₁ t₂: Term τ} (he: Eval₁ τ t₁ t₂): Halts t₁ ↔ Halts t₂ := sorry
-      theorem preservesTotality {τ: Ty} {t₁ t₂: Term τ} (he: Eval₁ τ t₁ t₂): Total τ t₁ ↔ Total τ t₂ := sorry
+      theorem preservesHalting {τ: Ty} {t₁ t₂: Term τ} (he: Eval₁ t₁ t₂): Halts t₁ ↔ Halts t₂ := sorry
+      theorem preservesTotality {τ: Ty} {t₁ t₂: Term τ} (he: Eval₁ t₁ t₂): Total t₁ ↔ Total t₂ := sorry
     end Eval₁
 
     namespace Eval
-      theorem deterministic {τ: Ty} {t t₁ t₂: Term τ}: Eval₁ τ t t₁ → Eval₁ τ t t₂ → t₁ = t₂ := sorry
-      theorem progress {τ: Ty} {t₁: Term τ}: IsValue τ t₁ ∨ ∃ t₂: Term τ, Eval₁ τ t₁ t₂ := sorry
+      theorem deterministic {τ: Ty} {t t₁ t₂: Term τ}: Eval₁ t t₁ → Eval₁ t t₂ → t₁ = t₂ := sorry
+      theorem progress {τ: Ty} {t₁: Term τ}: IsValue t₁ ∨ ∃ t₂: Term τ, Eval₁ t₁ t₂ := sorry
 
-      theorem preservesTotality {τ: Ty} {t₁ t₂: Term τ} (he: Eval τ t₁ t₂): Total τ t₁ ↔ Total τ t₂ := sorry
+      theorem preservesTotality {τ: Ty} {t₁ t₂: Term τ} (he: Eval t₁ t₂): Total t₁ ↔ Total t₂ := sorry
       theorem normalization {τ: Ty} {t: Term τ}: Halts t := sorry
     end Eval
   end Term
 
   namespace Top
     namespace Eval₁
-      theorem deterministic {τ: Ty} {t t₁ t₂: Top ρ τ}: Eval₁ τ t t₁ → Eval₁ τ t t₂ → t₁ = t₂ := sorry
-      theorem progress {τ: Ty} {t₁: Top ρ τ}: IsValue τ t₁ ∨ ∃ t₂: Top ρ τ, Eval₁ τ t₁ t₂ := sorry
+      theorem deterministic {τ: Ty} {t t₁ t₂: Top τ}: Eval₁ t t₁ → Eval₁ t t₂ → t₁ = t₂ := sorry
+      theorem progress {τ: Ty} {t₁: Top τ}: IsValue t₁ ∨ ∃ t₂: Top τ, Eval₁ t₁ t₂ := sorry
 
-      theorem preservesHalting {τ: Ty} {t₁ t₂: Top ρ τ} (he: Eval₁ τ t₁ t₂): Halts t₁ ↔ Halts t₂ := sorry
-      theorem preservesTotality {τ: Ty} {t₁ t₂: Top ρ τ} (he: Eval₁ τ t₁ t₂): Total τ t₁ ↔ Total τ t₂ := sorry
+      theorem preservesHalting {τ: Ty} {t₁ t₂: Top τ} (he: Eval₁ t₁ t₂): Halts t₁ ↔ Halts t₂ := sorry
+      theorem preservesTotality {τ: Ty} {t₁ t₂: Top τ} (he: Eval₁ t₁ t₂): Total τ t₁ ↔ Total τ t₂ := sorry
     end Eval₁
 
     namespace Eval
-      theorem deterministic {τ: Ty} {t t₁ t₂: Top ρ τ}: Eval₁ τ t t₁ → Eval₁ τ t t₂ → t₁ = t₂ := sorry
-      theorem progress {τ: Ty} {t₁: Top ρ τ}: IsValue τ t₁ ∨ ∃ t₂: Top ρ τ, Eval₁ τ t₁ t₂ := sorry
+      theorem progress {τ: Ty} {t₁: Top τ}: IsValue t₁ ∨ ∃ t₂: Top τ, Eval t₁ t₂ := sorry
 
-      theorem preservesTotality {τ: Ty} {t₁ t₂: Top ρ τ} (he: Eval τ t₁ t₂): Total τ t₁ ↔ Total τ t₂ := sorry
-      theorem normalization {τ: Ty} {t: Top ρ τ}: Halts t := sorry
+      theorem preservesTotality {τ: Ty} {t₁ t₂: Top τ} (he: Eval t₁ t₂): Total τ t₁ ↔ Total τ t₂ := sorry
+      theorem normalization {τ: Ty} {t: Top τ}: Halts t := sorry
     end Eval
   end Top
 end Total.Stlc.Lang.Annotated
